pulse/src/checker/Pulse.Checker.Rewrite.fst
@@ -140,6 +140,6 @@ let check
                  (T.moduleof (fstar_env g))
                  "Pulse.Checker.Rewrite.check_slprop_equiv_tac"
   in
-	let d = T_Rewrite _ p q p_typing equiv_p_q in
+	let d = T_Rewrite _ p q equiv_p_q in
   let (| c,d |) = match_comp_res_with_post_hint d post_hint in
 	prove_post_hint (try_frame_pre false pre_typing (| _,c,d |) res_ppname) post_hint t.range
