pulse/src/checker/Pulse.Elaborate.Core.fst
@@ -170,132 +170,7 @@ let rec elab_st_typing (#g:env)
                        (#c:comp)
                        (d:st_typing g t c)
   : GTot R.term (decreases d)
-  = match d with
-    | T_Abs _ x qual b _u body _c ty_typing body_typing ->
-      let ty = b.binder_ty in
-      let ppname = b.binder_ppname.name in
-      let body = elab_st_typing body_typing in
-      mk_abs_with_name ppname ty (elab_qual qual) (RT.close_term body x) //this closure should be provably redundant by strengthening the conditions on x
-
-    | T_ST _ t _ _
-    | T_STGhost _ t _ _ _ -> t
-
-    | T_Return _ c use_eq u ty t post _ _ _ _ ->
-      let rp = mk_abs ty R.Q_Explicit post in
-      (match c, use_eq with
-       | STT, true -> mk_stt_return u ty t rp
-       | STT, false -> mk_stt_return_noeq u ty t rp
-       | STT_Atomic, true -> mk_stt_atomic_return u ty t rp
-       | STT_Atomic, false -> mk_stt_atomic_return_noeq u ty t rp
-       | STT_Ghost, true -> mk_stt_ghost_return u ty t rp
-       | STT_Ghost, false -> mk_stt_ghost_return_noeq u ty t rp)
-
-    | T_Bind _ e1 e2 c1 c2 b x c e1_typing t_typing e2_typing bc ->
-      let e1 = elab_st_typing e1_typing in
-      let e2 = elab_st_typing e2_typing in
-      let ty1 = comp_res c1 in
-      elab_bind bc e1 (mk_abs_with_name b.binder_ppname.name ty1 R.Q_Explicit (RT.close_term e2 x))
-
-    | T_BindFn _ _ _ c1 c2 b x e1_typing _u t_typing e2_typing c2_typing ->
-      let e1 = elab_st_typing e1_typing in
-      let e2 = elab_st_typing e2_typing in
-      let ty1 = comp_res c1 in
-      RT.mk_let RT.pp_name_default e1 ty1 (RT.close_term e2 x)
-      
-    | T_Frame _ _ c frame _frame_typing e_typing ->
-      let e = elab_st_typing e_typing in
-      elab_frame c frame e
-      
-    | T_Equiv _ _ c1 c2 e_typing (ST_TotEquiv _ _ _ _ _ _) ->
-      let e = elab_st_typing e_typing in
-      e
-
-    | T_Equiv _ _ c1 c2 e_typing _ ->
-      let e = elab_st_typing e_typing in
-      elab_sub c1 c2 e
-
-    | T_Sub _ _ c1 c2 e_typing d_sub ->
-      let e = elab_st_typing e_typing in
-      let (| coercion, _ |) = elab_st_sub d_sub in
-      R.mk_e_app coercion [e]
-
-    | T_Lift _ _ c1 c2 e_typing lc ->
-      let e = elab_st_typing e_typing in
-      elab_lift lc e
-
-    | T_If _ b _ _ _ _ _ e1_typing e2_typing _c_typing ->
-      let re1 = elab_st_typing e1_typing in
-      let re2 = elab_st_typing e2_typing in
-      RT.mk_if b re1 re2
-
-    | T_Match _ _ _ sc _ _ _ _ _ brty  _ ->
-      let brs = elab_branches brty in
-      R.pack_ln (R.Tv_Match sc None brs)
-
-    | T_IntroPure _ p _ _ ->
-      let head = 
-        tm_pureapp (tm_fvar (as_fv (mk_pulse_lib_core_lid "intro_pure")))
-                       None
-                       p
-      in
-      let arg = (`()) in
-      R.mk_app head [(arg, elab_qual None)]
-
-    | T_ElimExists _ u t p _ d_t d_exists ->
-      mk_elim_exists u t (mk_abs t R.Q_Explicit p)
-
-    | T_IntroExists _ u b p e _ _ _ ->
-      let rt = b.binder_ty in
-      mk_intro_exists u rt (mk_abs rt R.Q_Explicit p) e
-
-    | T_While .. ->
-      admit ()
-      // let cond = elab_st_typing cond_typing in
-      // let body = elab_st_typing body_typing in
-      // mk_while inv (mk_abs bool_tm R.Q_Explicit post) cond body
-
-		| T_Rewrite _ p q _ _ ->
-		  mk_rewrite p q
-
-    | T_WithLocal _ _ init _ init_t c x _ _ _ body_typing ->
-      let rret_u = comp_u c in
-      let rret_t = comp_res c in
-      let rpre = comp_pre c in
-      let rpost = mk_abs rret_t R.Q_Explicit (comp_post c) in
-      let rbody = elab_st_typing body_typing in
-      let rbody = RT.close_term rbody x in
-      let rbody = mk_abs (mk_ref init_t) R.Q_Explicit rbody in
-      mk_withlocal rret_u init_t init rpre rret_t rpost rbody
-
-    | T_WithLocalUninit .. ->
-      admit ()
-
-    | T_WithLocalArray _ _ init len _ init_t c x _ _ _ _ body_typing ->
-      let rret_u = comp_u c in
-      let rret_t = comp_res c in
-      let rpre = comp_pre c in
-      let rpost = mk_abs rret_t R.Q_Explicit (comp_post c) in
-      let rbody = elab_st_typing body_typing in
-      let rbody = RT.close_term rbody x in
-      let rbody = mk_abs (mk_array init_t) R.Q_Explicit rbody in
-      mk_withlocalarray rret_u init_t init len rpre rret_t rpost rbody
-
-    | T_WithLocalArrayUninit .. ->
-      admit ()
-
-    | T_Admit _ c _ ->
-      let {u; res; pre; post} = st_comp_of_comp c in
-      let rpost = mk_abs res R.Q_Explicit post in
-      (match c with
-       | C_ST _ -> mk_stt_admit u res pre rpost
-       | C_STAtomic _ _ _ -> mk_stt_atomic_admit u res pre rpost
-       | C_STGhost _ _ -> mk_stt_ghost_admit u res pre rpost)
-    
-    | T_ForwardJumpLabel .. -> admit ()
-    | T_Goto .. -> admit ()
-
-    | T_Unreachable .. ->
-      `("IOU: elab_st_typing of T_Unreachable")
+  = RU.magic ()
 
 and elab_br (#g:env)
             (#c:comp_st)
@@ -304,9 +179,7 @@ and elab_br (#g:env)
             (#e:st_term)
             (d : br_typing g sc_u sc_ty sc p e c)
   : GTot R.branch (decreases d)
-  = let TBR _ _ _ _ _ _ _ _ bs _ _ _ ed = d in
-    let e = elab_st_typing ed in
-    (elab_pat p, e)
+  = RU.magic ()
 and elab_branches (#g:env)
                   (#c:comp_st)
                   (#sc_u:universe) (#sc_ty:typ) (#sc:term)
@@ -314,7 +187,4 @@ and elab_branches (#g:env)
                   (d : brs_typing g sc_u sc_ty sc brs c)
   : GTot (list R.branch)
         (decreases d)
-  = match d with
-    | TBRS_0 _ -> []
-    | TBRS_1 _ p e bd _ d' ->
-    elab_br bd :: elab_branches d'
+  = RU.magic ()
